interface/Finite_set.fst
@@ -1,0 +1,135 @@
+(*
+   Copyright 2008-2021 John Li, Jay Lorch, Rustan Leino, Alex Summers,
+   Dan Rosen, Nikhil Swamy, Microsoft Research, and contributors to
+   the Dafny Project
+
+   Licensed under the Apache License, Version 2.0 (the "License");
+   you may not use this file except in compliance with the License.
+   You may obtain a copy of the License at
+
+       http://www.apache.org/licenses/LICENSE-2.0
+
+   Unless required by applicable law or agreed to in writing, software
+   distributed under the License is distributed on an "AS IS" BASIS,
+   WITHOUT WARRANTIES OR CONDITIONS OF ANY KIND, either express or implied.
+   See the License for the specific language governing permissions and
+   limitations under the License.
+
+   Includes material from the Dafny project
+   (https://github.com/dafny-lang/dafny) which carries this license
+   information:
+
+     Created 9 February 2008 by Rustan Leino.
+     Converted to Boogie 2 on 28 June 2008.
+     Edited sequence axioms 20 October 2009 by Alex Summers.
+     Modified 2014 by Dan Rosen.
+     Copyright (c) 2008-2014, Microsoft.
+     Copyright by the contributors to the Dafny Project
+     SPDX-License-Identifier: MIT
+*)
+
+(**
+This module declares a type and functions used for modeling
+finite sets as they're modeled in Dafny.
+
+@summary Type and functions for modeling finite sets
+*)
+
+module Finite_set
+module FLT = FStar.List.Tot
+open FStar.FunctionalExtensionality
+
+let has_elements (#a: eqtype) (f: a ^-> bool) (xs: list a): prop =
+  forall x. f x == x `FLT.mem` xs
+
+let t (a:eqtype) = f:(a ^-> bool){exists xs. f `has_elements` xs}
+
+let rec remove_repeats (#a: eqtype) (xs: list a)
+: (ys: list a{list_nonrepeating ys /\ (forall y. FLT.mem y ys <==> FLT.mem y xs)}) =
+  match xs with
+  | [] -> []
+  | hd :: tl -> let tl' = remove_repeats tl in if FLT.mem hd tl then tl' else hd :: tl'
+
+let mem #a x s = s x
+
+let set_as_list (#a: eqtype) (s: t a): GTot (xs: list a{list_nonrepeating xs /\ (forall x. FLT.mem x xs = mem x s)}) =
+  remove_repeats (FStar.IndefiniteDescription.indefinite_description_ghost (list a) (fun xs -> forall x. FLT.mem x xs = mem x s))
+  
+let intro_set (#a: eqtype) (f: a ^-> bool) (xs: Ghost.erased (list a))
+: Pure (t a)
+    (requires f `has_elements` xs)
+    (ensures fun _ -> True)
+= Classical.exists_intro (fun xs -> f `has_elements` xs) xs;
+  f 
+  
+let empty #a = intro_set (on_dom a (fun _ -> false)) []
+
+let insert (#a: eqtype) (x: a) (s: t a): t a =
+  intro_set (on_dom _ (fun x' -> x = x' || s x')) (x :: set_as_list s)
+
+let singleton #a x = insert x empty
+let equal #a s1 s2 = feq s1 s2
+
+let rec union_lists (#a: eqtype) (xs: list a) (ys: list a) : (zs: list a{forall z. FLT.mem z zs <==> FLT.mem z xs \/ FLT.mem z ys}) =
+  match xs with
+  | [] -> ys
+  | hd :: tl -> hd :: union_lists tl ys
+  
+let union #a s1 s2 = intro_set (on_dom a (fun x -> s1 x || s2 x)) (union_lists (set_as_list s1) (set_as_list s2))
+
+let rec intersect_lists (#a: eqtype) (xs: list a) (ys: list a)
+: (zs: list a{forall z. FLT.mem z zs <==> FLT.mem z xs /\ FLT.mem z ys}) =
+  match xs with
+  | [] -> []
+  | hd :: tl -> let zs' = intersect_lists tl ys in if FLT.mem hd ys then hd :: zs' else zs'
+
+let intersection #a s1 s2 = intro_set (on_dom a (fun x -> s1 x && s2 x)) (intersect_lists (set_as_list s1) (set_as_list s2))
+
+//let complement #a s = F.on_dom a (fun x -> not (s x))
+
+let rec difference_lists (#a: eqtype) (xs: list a) (ys: list a)
+: (zs: list a{forall z. FLT.mem z zs <==> FLT.mem z xs /\ ~(FLT.mem z ys)}) =
+  match xs with
+  | [] -> []
+  | hd :: tl -> let zs' = difference_lists tl ys in if FLT.mem hd ys then zs' else hd :: zs'
+  
+let difference #a s1 s2 = intro_set (on_dom a (fun x -> s1 x && not (s2 x))) (difference_lists (set_as_list s1) (set_as_list s2))
+
+let rec filter_lists (#a: eqtype) (xs: list a) (p: a -> bool)
+: (zs: list a{forall z. FLT.mem z zs <==> FLT.mem z xs /\ p z}) =
+  match xs with
+  | [] -> []
+  | hd :: tl -> let zs' = filter_lists tl p in if p hd then hd::zs' else zs'
+  
+let filter #a s1 p = intro_set (on_dom a (fun x -> s1 x && p x)) (filter_lists (set_as_list s1) p)
+
+let rec remove_lists (#a: eqtype) (xs: list a) (x: a)
+: (zs: list a{forall z. FLT.mem z zs <==> FLT.mem z xs /\ z <> x}) =
+  match xs with
+  | [] -> []
+  | hd :: tl -> let zs' = remove_lists tl x in if hd = x then zs' else hd::zs'
+  
+let remove #a s1 y = intro_set (on_dom a (fun x -> s1 x && x <> y)) (remove_lists (set_as_list s1) y)
+
+[@"opaque_to_smt"]
+let cardinality (#a: eqtype) (s: t a) : GTot nat =
+  FLT.length (set_as_list s)
+
+let choose (#a: eqtype) (s: t a{exists x. mem x s}) : GTot (x: a{mem x s}) =
+  Cons?.hd (set_as_list s)
+  
+let mem_empty #a x = ()
+let equal_intro #a s1 s2 = ()
+let equal_intro' #a s1 s2 = ()
+let equal_elim #a s1 s2 = () 
+let insert_mem # a x s = ()
+let mem_subset #a s1 s2 = ()
+let subset_mem #a s1 s2 = ()
+let mem_union #a s1 s2 x = ()
+let mem_singleton #a x y = ()
+let mem_intersection #a s1 s2 x = ()
+let mem_complement #a s x = ()
+let mem_difference #a s1 s2 x = ()
+let mem_filter #a s p x = ()
+let mem_remove_x #a s x = ()
+let mem_remove_y #a s x y = ()
